universe 0 arrays

ulib/experimental/Steel.Array0.fsti
@@ -1,11 +1,6 @@
-module Steel.HigherArray0
+module Steel.Array0
 
-/// C arrays of universe 1 elements.
-/// 
-/// - Due to a limitation on the universe for selectors, no selector
-///   version can be defined for universe 1.
-/// - Due to F* universes not being cumulative, arrays of universe 0
-///   elements need to be defined in a separate module.
+/// C arrays of universe 0 elements, with selectors.
 
 module P = Steel.FractionalPermission
 module U32 = FStar.UInt32
@@ -14,19 +9,24 @@ open Steel.Memory
 open Steel.Effect.Atomic
 open Steel.Effect
 
-/// NOTE: This module is slated to have primitive Karamel extraction
-/// (except for definitions meant to be inlined.)
+/// NOTE: This module is defined on top of Steel.HigherArray0, so its
+/// definitions are all meant to be inlined and benefit from the
+/// latter module's primitive extraction. We seal it under an
+/// interface to avoid unpleasantly leaking the lifting of values
+/// of lower universes into the SMT context. Due to this interface,
+/// cross-module inlining must be enabled using F*'s --cmi option.
 
 /// An abstract type to represent a base array (whole allocation
 /// unit), exposed for proof purposes only
 [@@erasable]
-val base_t (elt: Type u#a) : Tot Type0
+val base_t (elt: Type0) : Tot Type0
 val base_len (#elt: Type) (b: base_t elt) : GTot nat
 
 /// An abstract type to represent a C pointer, as a base and an offset
 /// into its base
-[@@noextract_to "krml"] // primitive
-val ptr (elt: Type u#a) : Type0
+inline_for_extraction
+[@@noextract_to "krml"]
+val ptr (elt: Type0) : Type0
 val base (#elt: Type) (p: ptr elt) : Tot (base_t elt)
 val offset (#elt: Type) (p: ptr elt) : Ghost nat (requires True) (ensures (fun offset -> offset <= base_len (base p)))
 val ptr_base_offset_inj (#elt: Type) (p1 p2: ptr elt) : Lemma
@@ -45,7 +45,7 @@ val ptr_base_offset_inj (#elt: Type) (p1 p2: ptr elt) : Lemma
 /// record type.
 inline_for_extraction
 [@@noextract_to "krml"]
-let array (elt: Type u#a) : Tot Type0 =
+let array (elt: Type0) : Tot Type0 =
   (p: ptr elt & (length: Ghost.erased nat {offset p + length <= base_len (base p)}))
 
 /// This will extract to "let p = a"
@@ -62,11 +62,9 @@ let length (#elt: Type) (a: array elt) : GTot nat =
   dsnd a
 
 /// A Steel separation logic heap predicate to describe that an array
-/// a points to some element sequence s with some permission p.  vprop
-/// limits the universe to at most 1 (because of the universe of the
-/// heap.)
+/// a points to some element sequence s with some permission p.
 val pts_to
-  (#elt: Type u#1) (a: array elt)
+  (#elt: Type0) (a: array elt)
   ([@@@ smt_fallback ] p: P.perm)
   ([@@@ smt_fallback ] s: Seq.seq elt)
 : Tot vprop
@@ -75,7 +73,7 @@ val pts_to
 /// of the element sequence it points to
 val pts_to_length
   (#opened: _)
-  (#elt: Type u#1) (a: array elt)
+  (#elt: Type0) (a: array elt)
   (p: P.perm)
   (s: Seq.seq elt)
 : SteelGhost unit opened
@@ -84,31 +82,51 @@ val pts_to_length
     (fun _ -> True)
     (fun _ _ _ -> Seq.length s == length a)
 
-/// An injectivity property, needed only to define a selector.  Such a
-/// selector can be only defined in universe 0, and universes are not
-/// cumulative, so we need to define a separate module for arrays of
-/// universe 0 elements with selectors, reusing definitions from this
-/// interface, but we do not want to use `friend`.
-val pts_to_inj
-  (#elt: Type u#1) (a: array elt)
-  (p1: P.perm)
-  (s1: Seq.seq elt)
-  (p2: P.perm)
-  (s2: Seq.seq elt)
-  (m: mem)
-: Lemma
-  (requires (
-    interp (hp_of (pts_to a p1 s1)) m /\
-    interp (hp_of (pts_to a p2 s2)) m
-  ))
-  (ensures (
-    s1 == s2
-  ))
+/// A selector version
+val varrayp_hp
+  (#elt: Type0) (a: array elt) (p: P.perm)
+: Tot (slprop u#1)
+
+val varrayp_sel
+  (#elt: Type) (a: array elt) (p: P.perm)
+: Tot (selector (Seq.lseq elt (length a)) (varrayp_hp a p))
+
+[@__steel_reduce__] // for t_of
+let varrayp
+  (#elt: Type) (a: array elt) (p: P.perm)
+: Tot vprop
+= VUnit ({
+    hp = varrayp_hp a p;
+    t = _;
+    sel = varrayp_sel a p;
+  })
+
+val intro_varrayp
+  (#opened: _) (#elt: Type) (a: array elt) (p: P.perm) (s: Seq.seq elt)
+: SteelGhost unit opened
+    (pts_to a p s)
+    (fun _ -> varrayp a p)
+    (fun _ -> True)
+    (fun _ _ h' ->
+      h' (varrayp a p) == s
+    )
+
+val elim_varrayp
+  (#opened: _) (#elt: Type) (a: array elt) (p: P.perm)
+: SteelGhost (Ghost.erased (Seq.seq elt)) opened
+    (varrayp a p)
+    (fun res -> pts_to a p res)
+    (fun _ -> True)
+    (fun h res _ ->
+      Ghost.reveal res == h (varrayp a p)
+    )
 
 /// Allocating a new array of size n, where each cell is initialized
-/// with value x
-[@@noextract_to "krml"] // primitive
-val alloc
+/// with value x. We define the non-selector version of this operation
+/// (and others) with a _pt suffix in the name.
+inline_for_extraction
+[@@noextract_to "krml"]
+val alloc_pt
   (#elt: Type)
   (x: elt)
   (n: U32.t)
@@ -118,10 +136,28 @@ val alloc
     (fun _ -> True)
     (fun _ a _ -> length a == U32.v n)
 
+inline_for_extraction
+[@@noextract_to "krml"]
+let alloc
+  (#elt: Type)
+  (x: elt)
+  (n: U32.t)
+: Steel (array elt)
+    emp
+    (fun a -> varrayp a P.full_perm)
+    (fun _ -> True)
+    (fun _ a h' ->
+      length a == U32.v n /\
+      h' (varrayp a P.full_perm) == Seq.create (U32.v n) x
+    )
+= let res = alloc_pt x n in
+  intro_varrayp res P.full_perm _;
+  return res
+
 /// Sharing and gathering permissions on an array. Those only
 /// manipulate permissions, so they are nothing more than stateful
 /// lemmas.
-val share
+val share_pt
   (#opened: _)
   (#elt: Type)
   (#x: Seq.seq elt)
@@ -133,7 +169,25 @@ val share
     (fun _ -> p == p1 `P.sum_perm` p2)
     (fun _ _ _ -> True)
 
-val gather
+let share
+  (#opened: _)
+  (#elt: Type)
+  (a: array elt)
+  (p p1 p2: P.perm)
+: SteelGhost unit opened
+    (varrayp a p)
+    (fun _ -> varrayp a p1 `star` varrayp a p2)
+    (fun _ -> p == p1 `P.sum_perm` p2)
+    (fun h _ h' ->
+      h' (varrayp a p1) == h (varrayp a p) /\
+      h' (varrayp a p2) == h (varrayp a p)
+    )
+= let _ = elim_varrayp a p in
+  share_pt a p p1 p2;
+  intro_varrayp a p1 _;
+  intro_varrayp a p2 _
+
+val gather_pt
   (#opened: _)
   (#elt: Type)
   (a: array elt)
@@ -145,10 +199,30 @@ val gather
     (fun _ -> True)
     (fun _ _ _ -> x1 == x2)
 
+let gather
+  (#opened: _)
+  (#elt: Type)
+  (a: array elt)
+  (p1: P.perm)
+  (p2: P.perm)
+: SteelGhost unit opened
+    (varrayp a p1 `star` varrayp a p2)
+    (fun _ -> varrayp a (p1 `P.sum_perm` p2))
+    (fun _ -> True)
+    (fun h _ h' ->
+      h' (varrayp a (p1 `P.sum_perm` p2)) == h (varrayp a p1) /\
+      h' (varrayp a (p1 `P.sum_perm` p2)) == h (varrayp a p2)
+    )
+= let _ = elim_varrayp a p1 in
+  let _ = elim_varrayp a p2 in
+  gather_pt a p1 p2;
+  intro_varrayp a _ _
+
 /// Reading the i-th element of an array a.
 /// TODO: we should also provide an atomic version for small types.
-[@@noextract_to "krml"] // primitive
-val index
+inline_for_extraction
+[@@noextract_to "krml"]
+val index_pt
   (#t: Type) (#p: P.perm)
   (a: array t)
   (#s: Ghost.erased (Seq.seq t))
@@ -159,10 +233,32 @@ val index
     (fun _ -> U32.v i < length a)
     (fun _ res _ -> U32.v i < Seq.length s /\ res == Seq.index s (U32.v i))
 
+inline_for_extraction
+[@@noextract_to "krml"]
+let index
+  (#t: Type) (#p: P.perm)
+  (a: array t)
+  (i: U32.t)
+: Steel t
+    (varrayp a p)
+    (fun _ -> varrayp a p)
+    (fun _ -> U32.v i < length a)
+    (fun h res h' ->
+      let s = h (varrayp a p) in
+      h' (varrayp a p) == s /\
+      U32.v i < Seq.length s /\
+      res == Seq.index s (U32.v i)
+    )
+= let _ = elim_varrayp a p in
+  let res = index_pt a i in
+  intro_varrayp a _ _;
+  return res
+
 /// Writing the value v at the i-th element of an array a.
 /// TODO: we should also provide an atomic version for small types.
+inline_for_extraction
 [@@noextract_to "krml"]
-val upd
+val upd_pt
   (#t: Type)
   (a: array t)
   (#s: Ghost.erased (Seq.seq t))
@@ -172,6 +268,25 @@ val upd
 : SteelT unit
     (pts_to a P.full_perm s)
     (fun res -> pts_to a P.full_perm (Seq.upd s (U32.v i) v))
+
+inline_for_extraction
+[@@noextract_to "krml"]
+let upd
+  (#t: Type)
+  (a: array t)
+  (i: U32.t)
+  (v: t)
+: Steel unit
+    (varrayp a P.full_perm)
+    (fun _ -> varrayp a P.full_perm)
+    (fun _ ->  U32.v i < length a)
+    (fun h _ h' ->
+      U32.v i < length a /\
+      h' (varrayp a P.full_perm) == Seq.upd (h (varrayp a P.full_perm)) (U32.v i) v
+    )
+= let _ = elim_varrayp a _ in
+  upd_pt a i () v;
+  intro_varrayp a _ _
 
 /// An array a1 is adjacent to an array a2 if and only if they have
 /// the same base array and the end of a1 coincides with the beginning
@@ -206,7 +321,7 @@ let merge_into (#elt: Type) (a1 a2 a: array elt) : Tot prop =
   merge a1 a2 == a
 
 /// Spatial merging of two arrays, expressed in terms of `merge`.
-val ghost_join
+val ghost_join_pt
   (#opened: _)
   (#elt: Type)
   (#x1 #x2: Seq.seq elt)
@@ -217,6 +332,24 @@ val ghost_join
     (pts_to a1 p x1 `star` pts_to a2 p x2)
     (fun res -> pts_to (merge a1 a2) p (x1 `Seq.append` x2))
 
+let ghost_join
+  (#opened: _)
+  (#elt: Type)
+  (#p: P.perm)
+  (a1 a2: array elt)
+  (sq: squash (adjacent a1 a2))
+: SteelGhost unit opened
+    (varrayp a1 p `star` varrayp a2 p)
+    (fun res -> varrayp (merge a1 a2) p)
+    (fun _ -> True)
+    (fun h _ h' ->
+      h' (varrayp (merge a1 a2) p) == h (varrayp a1 p) `Seq.append` h (varrayp a2 p)
+    )
+= let _ = elim_varrayp a1 p in
+  let _ = elim_varrayp a2 p in
+  ghost_join_pt a1 a2 ();
+  intro_varrayp (merge a1 a2) _ _
+
 /// Spatial merging, combining the use of `merge` and the call to the
 /// stateful lemma. Since the only operations are calls to stateful
 /// lemmas and pure computations, the overall computation is atomic
@@ -225,7 +358,7 @@ val ghost_join
 /// "let res = a1"
 inline_for_extraction // this will extract to "let res = a1"
 [@@noextract_to "krml"]
-let join
+let join_pt
   (#opened: _)
   (#elt: Type)
   (#x1 #x2: Ghost.erased (Seq.seq elt))
@@ -237,11 +370,33 @@ let join
     (fun res -> pts_to res p (x1 `Seq.append` x2))
     (fun _ -> adjacent a1 a2)
     (fun _ res _ -> merge_into a1 a2 res)
-= ghost_join a1 a2 ();
+= ghost_join_pt a1 a2 ();
   let res = merge a1 a2 in
   change_equal_slprop
     (pts_to (merge a1 (Ghost.reveal a2)) p (x1 `Seq.append` x2))
     (pts_to res p (x1 `Seq.append` x2));
+  return res
+
+inline_for_extraction // this will extract to "let res = a1"
+[@@noextract_to "krml"]
+let join
+  (#opened: _)
+  (#elt: Type)
+  (#p: P.perm)
+  (a1: array elt)
+  (a2: Ghost.erased (array elt))
+: SteelAtomicBase (array elt) false opened Unobservable
+    (varrayp a1 p `star` varrayp a2 p)
+    (fun res -> varrayp res p)
+    (fun _ -> adjacent a1 a2)
+    (fun h res h' ->
+      merge_into a1 a2 res /\
+      h' (varrayp res p) == h (varrayp a1 p) `Seq.append` h (varrayp a2 p)
+    )
+= let _ = elim_varrayp a1 _ in
+  let _ = elim_varrayp a2 _ in
+  let res = join_pt a1 a2 in
+  intro_varrayp res _ _;
   return res
 
 /// Computing the left-hand-side part of splitting an array a at
@@ -260,6 +415,7 @@ let split_l (#elt: Type) (a: array elt)
 /// offset off.  TODO: replace this with a Ghost definition and a
 /// SteelAtomicBase Unobservable operation with the corresponding
 /// permission.
+inline_for_extraction
 [@@noextract_to "krml"]
 val ptr_shift
   (#elt: Type)
@@ -284,10 +440,10 @@ let split_r (#elt: Type) (a: array elt)
 = (| ptr_shift (ptr_of a) i, Ghost.hide (length a - U32.v i) |)
 
 /// Splitting an array a at offset i, as a stateful lemma expressed in
-/// terms of split_l, split_r. This stateful lemma returns a proof
-/// that offset i is in bounds of the value sequence, which is needed to
-/// typecheck the post-resource.
-val ghost_split
+/// terms of split_l, split_r. In the non-selector case, this stateful
+/// lemma returns a proof that offset i is in bounds of the value
+/// sequence, which is needed to typecheck the post-resource.
+val ghost_split_pt
   (#opened: _)
   (#elt: Type)
   (#x: Seq.seq elt)
@@ -303,6 +459,29 @@ val ghost_split
     (fun _ res _ ->
       x == Seq.append (Seq.slice x 0 (U32.v i)) (Seq.slice x (U32.v i) (Seq.length x))
     )
+
+let ghost_split
+  (#opened: _)
+  (#elt: Type)
+  (#p: P.perm)
+  (a: array elt)
+  (i: U32.t { U32.v i <= length a })
+: SteelGhost unit opened
+    (varrayp a p)
+    (fun _ -> varrayp (split_l a i) p `star` varrayp (split_r a i) p)
+    (fun _ -> True)
+    (fun h _ h' ->
+      let x = h (varrayp a p) in
+      let xl = Seq.slice x 0 (U32.v i) in
+      let xr = Seq.slice x (U32.v i) (Seq.length x) in
+      h' (varrayp (split_l a i) p) == xl /\
+      h' (varrayp (split_r a i) p) == xr /\
+      x == Seq.append xl xr
+    )
+= let _ = elim_varrayp a _ in
+  ghost_split_pt a i;
+  intro_varrayp (split_l a i) _ _;
+  intro_varrayp (split_r a i) _ _
 
 /// NOTE: we could implement a SteelAtomicBase Unobservable "split"
 /// operation, just like "join", but we don't want it to return a pair
